feat: type refs in objects and types

LeanPy/Data/FrozenRef.lean
@@ -1,22 +1,25 @@
 /-
 Copyright (c) 2025 Mac Malone. All rights reserved.
 Released under the Apache 2.0 license as described in the file LICENSE.
-syntax Authors Mac Malone
+Authors: Mac Malone
 -/
 
 namespace LeanPy
 
 /-- An immutable value equipped with its runtime address. -/
 structure FrozenRef (α : Type u) where
-  private noncomputableMk ::
-    private noncomputableAddr : USize
-    private noncomputableData : α
+  -- TODO: Not `private` due to https://github.com/leanprover/lean4/issues/10789
+  innerMk ::
+    private innerAddr : USize
+    private innerData : α
   deriving Nonempty
 
 namespace FrozenRef
 
 noncomputable def mk (addr : USize) (data : α) : FrozenRef α :=
-  noncomputableMk addr data
+  innerMk addr data
+
+attribute [deprecated "Do not use `innerMk` directly." (since := "always")] innerMk
 
 private unsafe def dataImpl (self : FrozenRef α) : α :=
   unsafeCast self
@@ -24,10 +27,12 @@ private unsafe def dataImpl (self : FrozenRef α) : α :=
 /-- The addressed data. -/
 @[implemented_by dataImpl]
 def data (self : FrozenRef α) : α :=
-  self.noncomputableData
+  self.innerData
 
 @[simp] theorem data_mk : data (mk n a) = a := by
   simp [mk, data]
+
+instance : CoeOut (FrozenRef α) α := ⟨data⟩
 
 @[inline] private unsafe def addrImpl (self : FrozenRef α) : USize :=
   ptrAddrUnsafe self
@@ -35,7 +40,7 @@ def data (self : FrozenRef α) : α :=
 /-- The address of `data`. In the case of a scalar, this is its boxed value. -/
 @[implemented_by addrImpl]
 def addr (self : FrozenRef α) : USize :=
-  self.noncomputableAddr
+  self.innerAddr
 
 @[simp] theorem addr_mk : addr (mk n a) = n := by
   simp [mk, addr]
@@ -45,6 +50,37 @@ theorem eq_iff : a = b ↔ addr a = addr b ∧ data a = data b := by
 
 @[simp] theorem mk_addr_data : mk (addr r) (data r) = r := by
   simp [eq_iff]
+
+@[simp] theorem mk_eq_iff : mk a₁ d₁ = mk a₂ d₂ ↔ a₁ = a₂ ∧ d₁ = d₂ := by
+  simp [eq_iff]
+
+noncomputable def null (a : α) : FrozenRef α :=
+  .mk 0 a
+
+@[inline] private unsafe def castImpl
+  (self : FrozenRef α) (_ : self.data = a)
+: FrozenRef α := unsafeCast self
+
+set_option linter.unusedVariables.funArgs false in
+/--
+Casts the reference's data to equivalent value in the logic.
+
+This can restore definitional equalities for the data
+after a reference has been created via an opaque definition.
+-/
+@[implemented_by castImpl]
+abbrev cast
+  (self : FrozenRef α) (h : self.data = a)
+: FrozenRef α := {self with innerData := a}
+
+@[simp] theorem cast_def : cast self h = self := by
+  cases self; simp only [data] at h; simp [cast, h]
+
+@[inline, elab_as_elim, cases_eliminator, induction_eliminator]
+def elim
+  {α : Type u} {motive : FrozenRef α → Sort v} (self : FrozenRef α)
+  (mk : (addr : USize) → (data : α) → motive (mk addr data))
+: motive self := mk self.addr self.data
 
 end FrozenRef
 
