LeanPy/Data/NonScalarRef.lean
@@ -1,7 +1,7 @@
 /-
 Copyright (c) 2025 Mac Malone. All rights reserved.
 Released under the Apache 2.0 license as described in the file LICENSE.
-syntax Authors Mac Malone
+Authors: Mac Malone
 -/
 import LeanPy.Data.FrozenRef
 
@@ -13,7 +13,9 @@ structure NonScalarRef (α : Type u) where
 
 namespace NonScalarRef
 
-@[inline] def addr (n : NonScalarRef α) : USize :=
+instance : Coe (NonScalarRef α) (FrozenRef α) := ⟨NonScalarRef.toFrozenRef⟩
+
+abbrev addr (n : NonScalarRef α) : USize :=
   n.toFrozenRef.addr
 
 @[simp] theorem addr_mk : addr (mk a h) = a.addr := rfl
@@ -23,7 +25,7 @@ namespace NonScalarRef
 @[simp] theorem toNat_addr_mod_two : (addr a).toNat % 2 = 0 := by
   simpa [← USize.toNat_inj, -addr_mod_two] using addr_mod_two
 
-@[inline] def data (n : NonScalarRef α) : α :=
+abbrev data (n : NonScalarRef α) : α :=
   n.toFrozenRef.data
 
 @[simp] theorem data_mk : data (mk a h) = a.data := rfl
