LeanPy/Data/Object/Data.lean
@@ -1,0 +1,46 @@
+/-
+Copyright (c) 2025 Mac Malone. All rights reserved.
+Released under the Apache 2.0 license as described in the file LICENSE.
+Authors: Mac Malone
+-/
+
+namespace LeanPy
+
+/-- The name of an object's Lean data type. -/
+abbrev DataKind := Lean.Name
+
+/-- Dynamic data index by a `DataKind`. -/
+structure ObjectData where
+  private innerMk ::
+    private innerKind : DataKind
+    private innerValue : NonScalar
+  deriving Nonempty
+
+export TypeName (typeName)
+
+instance : TypeName Unit := unsafe (.mk _ ``Unit)
+
+namespace ObjectData
+
+@[inline] private unsafe def mkImpl [TypeName α] (a : α) : ObjectData :=
+  unsafeCast a
+
+@[implemented_by mkImpl]
+def mk [TypeName α] (a : α) : ObjectData :=
+  {innerKind := typeName α, innerValue := unsafe unsafeCast a}
+
+noncomputable def kind (self : ObjectData) : DataKind :=
+  self.innerKind
+
+@[simp] theorem kind_mk  [TypeName α] {a : α} : kind (mk a) = typeName α := rfl
+
+@[inline] private unsafe def getImpl
+  [Nonempty α] [TypeName α]
+  (self : ObjectData) (_ : self.kind = typeName α) : α
+:= unsafeCast self
+
+@[implemented_by getImpl]
+opaque get
+  [Nonempty α] [TypeName α]
+  (self : ObjectData) (h : self.kind = typeName α)
+: α
