LeanPy/Data/Object/ObjectType.lean
@@ -1,0 +1,23 @@
+/-
+Copyright (c) 2025 Mac Malone. All rights reserved.
+Released under the Apache 2.0 license as described in the file LICENSE.
+Authors: Mac Malone
+-/
+import LeanPy.Data.Object.Type
+
+namespace LeanPy
+
+def objectTypeDoc : String := "\
+  The base class of the class hierarchy.\n\
+  \n\
+  When called, it accepts no arguments and returns a new featureless\n\
+  instance that has no instance attributes and cannot be given any.\n\
+  "
+
+@[reducible] def objectType : TypeSpec where
+  name := "object"
+  doc? := some objectTypeDoc
+
+initialize objectTypeRef' : DTypeSpecRef objectType ← mkDTypeSpecRef _
+
+abbrev objectTypeRef : TypeSpecRef := objectTypeRef'.toTypeSpecRef
