LeanPy/Data/Object/ObjectTypes.lean
@@ -1,0 +1,105 @@
+/-
+Copyright (c) 2025 Mac Malone. All rights reserved.
+Released under the Apache 2.0 license as described in the file LICENSE.
+Authors: Mac Malone
+-/
+import LeanPy.Data.IntRef
+import LeanPy.Data.StringRef
+import LeanPy.Data.MutableRef
+import LeanPy.Data.Object.ObjectType
+
+/-!
+Built-in types inheriting directly from `object`. These are in a separate
+file from their parent due to `initialize` limitations.
+-/
+
+namespace LeanPy
+
+/-! ## `NoneType` -/
+
+@[reducible] def noneType : TypeSpec where
+  name := "NoneType"
+  base? := some objectTypeRef
+  IsValidObject id data :=
+    id = .none ∧ data = .mk ()
+
+initialize noneTypeRef' : DTypeSpecRef noneType ← mkDTypeSpecRef _
+
+abbrev noneTypeRef : TypeSpecRef := noneTypeRef'.toTypeSpecRef
+
+/-! ## `type` -/
+
+def typeTypeDoc : String := "\
+  type(object) -> the object's type\n\
+  type(name, bases, dict, **kwds) -> a new type\
+  "
+
+@[reducible] def typeType : TypeSpec where
+  name := "type"
+  doc? := some typeTypeDoc
+  isTypeSubclass := true
+  base? := some objectTypeRef
+  IsValidObject id data :=
+    id.isNonScalar ∧ data.kind = typeName TypeSpecRef
+
+initialize typeTypeRef' : DTypeSpecRef typeType ← mkDTypeSpecRef _
+
+abbrev typeTypeRef : TypeSpecRef := typeTypeRef'.toTypeSpecRef
+
+/-! ## `str` -/
+
+def strTypeDoc : String := "\
+  str(object='') -> str\n\
+  str(bytes_or_buffer[, encoding[, errors]]) -> str\n\
+  \n\
+  Create a new string object from the given object. If encoding or\n\
+  errors is specified, then the object must expose a data buffer\n\
+  that will be decoded using the given encoding and error handler.\n\
+  Otherwise, returns the result of object.__str__() (if defined)\n\
+  or repr(object).\n\
+  encoding defaults to sys.getdefaultencoding().\n\
+  errors defaults to 'strict'.\
+  "
+
+@[reducible] def strType : TypeSpec where
+  name := "str"
+  doc? := some strTypeDoc
+  isStrSubclass := true
+  base? := some objectTypeRef
+  IsValidObject id data :=
+    id.isNonScalar ∧ data.kind = typeName StringRef
+
+initialize strTypeRef' : DTypeSpecRef strType ← mkDTypeSpecRef _
+
+abbrev strTypeRef : TypeSpecRef := strTypeRef'.toTypeSpecRef
+
+/-! ## `int` -/
+
+def intTypeDoc : String := "\
+  int([x]) -> integer\n\
+  int(x, base=10) -> integer\n\
+  \n\
+  Convert a number or string to an integer, or return 0 if no arguments\n\
+  are given.  If x is a number, return x.__int__().  For floating point\n\
+  numbers, this truncates towards zero.\n\
+  \n\
+  If x is not a number or if base is given, then x must be a string,\n\
+  bytes, or bytearray instance representing an integer literal in the\n\
+  given base.  The literal can be preceded by '+' or '-' and be surrounded\n\
+  by whitespace.  The base defaults to 10.  Valid bases are 0 and 2-36.\n\
+  Base 0 means to interpret the base from the string as an integer literal.\n\
+  >>> int('0b100', base=0)\n\
+  4\
+  "
+
+@[reducible] def intType : TypeSpec where
+  name := "int"
+  doc? := some intTypeDoc
+  isIntSubclass := true
+  base? := some objectTypeRef
+  IsValidObject _ data :=
+    data.kind = typeName IntRef -- TODO: id.isInt
+
+initialize intTypeRef' : DTypeSpecRef intType ← mkDTypeSpecRef _
+
+abbrev intTypeRef : TypeSpecRef := intTypeRef'.toTypeSpecRef
