LeanPy/Data/Object/ObjectTypes2.lean
@@ -1,0 +1,39 @@
+/-
+Copyright (c) 2025 Mac Malone. All rights reserved.
+Released under the Apache 2.0 license as described in the file LICENSE.
+Authors: Mac Malone
+-/
+import LeanPy.Data.IntRef
+import LeanPy.Data.StringRef
+import LeanPy.Data.MutableRef
+import LeanPy.Data.Object.ObjectTypes
+
+/-!
+Built-in types inheriting from a direct subclass of `object`. These are in a
+separate file from their parents due to `initialize` limitations.
+-/
+
+namespace LeanPy
+
+def boolTypeDoc : String := "\
+  bool(x) -> bool\n\
+  \n\
+  Returns True when the argument x is true, False otherwise.\n\
+  The builtins True and False are the only two instances of the class bool.\n\
+  The class bool is a subclass of the class int, and cannot be subclassed.\
+  "
+
+@[reducible] def boolType : TypeSpec where
+  name := "bool"
+  doc? := some boolTypeDoc
+  base? := some intTypeRef
+  isIntSubclass := true
+  IsValidObject id data :=
+    (id = .false ∨ id = .true) ∧
+    (id = .false → data = .mk (0 : IntRef)) ∧
+    (id = .true → data = .mk (1 : IntRef)) ∧
+    data.kind = typeName IntRef -- redundant, but makes `simp_all` work bellow
+
+initialize boolTypeRef' : DTypeSpecRef boolType ← mkDTypeSpecRef _
+
+abbrev boolTypeRef : TypeSpecRef := boolTypeRef'.toTypeSpecRef
