LeanPy/Data/Object/Type.lean
@@ -1,0 +1,260 @@
+/-
+Copyright (c) 2025 Mac Malone. All rights reserved.
+Released under the Apache 2.0 license as described in the file LICENSE.
+Authors: Mac Malone
+-/
+import LeanPy.Data.Object.Id
+import LeanPy.Data.Object.Data
+
+namespace LeanPy
+
+/-! ## Object Type -/
+
+/-- A Python type. -/
+structure TypeSpec where
+  /-- The type's name -/
+  name : String
+  /-- The type's documentation string or `none` if undefined. -/
+  doc? : Option String := none
+  /-- The type's parent. -/
+  base? : Option (FrozenRef TypeSpec) := none
+  /--
+  Is this type is a legal base for other types.
+  If `false`, this type cannot be legally subtyped.
+
+  Equivalent in functionality to CPython's `Py_TPFLAGS_BASETYPE`.
+  -/
+  isBaseType : Bool := true
+  /--
+  Is this a subclass of `type`?
+
+  Equivalent in functionality to CPython's `Py_TPFLAGS_TYPE_SUBCLASS`.
+  -/
+  isTypeSubclass : Bool := false
+  /--
+  Is this a subclass of `str`?
+
+  Equivalent in functionality to CPython's `Py_TPFLAGS_UNICODE_SUBCLASS`.
+  -/
+  isStrSubclass : Bool := false
+  /--
+  Is this a subclass of `int`?
+
+  Equivalent in functionality to CPython's `Py_TPFLAGS_LONG_SUBCLASS`.
+  -/
+  isIntSubclass : Bool := false
+  /--
+  Returns whether the field combination could be a valid object of this type.
+
+  This can be an over-approximation. That is, it may hold for objects
+  which are not objects of this type.
+  -/
+  IsValidObject (id : ObjectId) (data : ObjectData) : Prop := True
+  deriving Nonempty
+
+namespace TypeSpec
+
+/-- The type's method resolution order. -/
+@[inline] def mro (self : TypeSpec) : List TypeSpec :=
+  self :: match self with
+    | {base? := none, ..} => []
+    | {base? := some base, ..} => mro base.data
+
+@[inline] def baseMro (self : TypeSpec) : List TypeSpec :=
+  match self with
+  | {base? := none, ..} => []
+  | {base? := some base, ..} => mro base.data
+
+theorem mro_def : mro self = self :: baseMro self := by
+  unfold mro baseMro; rfl
+
+theorem mem_mro_iff : ty ∈ mro self ↔ ty = self ∨ ty ∈ baseMro self := by
+  simp [mro_def]
+
+@[simp] theorem self_mem_mro : self ∈ mro self := by
+  simp [mro_def]
+
+@[simp] theorem baseMro_subset_mro : baseMro self ⊆ mro self := by
+  simp [mro_def]
+
+theorem mem_mro_of_mem_baseMro : ty ∈ baseMro self → ty ∈ mro self :=
+  List.subset_def.mp baseMro_subset_mro
+
+private theorem mem_mro_trans :
+  ty₁ ∈ mro ty₂ → ty₂ ∈ mro self → ty₁ ∈ mro self
+:= by
+  revert ty₂
+  let {base?, ..} := self
+  cases base? with
+  | none =>
+    intro ty₂ h₁
+    simp only [mro, List.mem_cons, List.not_mem_nil, or_false]
+    intro h₂
+    simpa [h₂, mro] using h₁
+  | some base =>
+    intro ty₂ h₁
+    simp only [mro, List.mem_cons]
+    intro h₂
+    cases h₂ with
+    | inl h₂ => simpa [h₂, mro] using h₁
+    | inr h₂ => exact Or.inr <| mem_mro_trans h₁ h₂
+
+def IsSubtype (self other : TypeSpec) : Prop :=
+  other ∈ self.mro
+
+instance : HasSubset TypeSpec := ⟨TypeSpec.IsSubtype⟩
+
+theorem subset_iff_mem_mro : a ⊆ b ↔ b ∈ mro a := Iff.rfl
+
+@[simp] theorem subset_rfl {self : TypeSpec} : self ⊆ self :=  self_mem_mro
+
+theorem subset_trans {a b c : TypeSpec} : a ⊆ b → b ⊆ c → a ⊆ c  := by
+  simp only [subset_iff_mem_mro]
+  exact fun h₁ h₂ => mem_mro_trans h₂ h₁
+
+end TypeSpec
+
+/-! ## Object Type Ref -/
+
+abbrev TypeSpecRef := FrozenRef TypeSpec
+
+noncomputable instance : SizeOf TypeSpecRef :=
+  inferInstanceAs (SizeOf (FrozenRef TypeSpec))
+
+namespace TypeSpecRef
+
+instance : TypeName TypeSpecRef := unsafe (.mk _ ``TypeSpecRef)
+
+/-- The type's method resolution order. -/
+@[inline] def mro (self : TypeSpecRef) : List TypeSpecRef :=
+  self :: go self.data
+where go self :=
+  match self with
+  | {base? := none, ..} => []
+  | {base? := some base, ..} => mro base
+
+@[inline] def baseMro (self : TypeSpecRef) : List TypeSpecRef :=
+  match self.data with
+  | {base? := none, ..} => []
+  | {base? := some base, ..} => mro base
+
+instance : SizeOf TypeSpecRef := ⟨(·.baseMro.length)⟩
+
+@[simp] theorem sizeOf_def {self : TypeSpecRef} :
+  sizeOf self = self.baseMro.length
+:= rfl
+
+theorem mro_def : mro self = self :: baseMro self := by
+  unfold mro baseMro mro.go; simp
+
+@[simp] theorem length_mro : (mro self).length = self.baseMro.length + 1 := by
+  simp [mro_def]
+
+theorem mem_mro_iff : ty ∈ mro self ↔ ty = self ∨ ty ∈ baseMro self := by
+  simp [mro_def]
+
+@[simp] theorem self_mem_mro : self ∈ mro self := by
+  simp [mro_def]
+
+@[simp] theorem baseMro_subset_mro : baseMro self ⊆ mro self := by
+  simp [mro_def]
+
+private theorem sup_mem_sub :
+  sup ∈ mro sub → ∀ {ty}, ty ∈ mro sup → ty ∈ mro sub
+:= by
+  simp only [mem_mro_iff]
+  match h_sub:sub.data with
+  | {base? := none, ..} =>
+    simp only [baseMro, h_sub, List.not_mem_nil, or_false]
+    intro sup_eq_sub
+    intro ty
+    simp [sup_eq_sub, h_sub]
+  | {base? := some base, ..} =>
+    have sub_baseMro : sub.baseMro = mro base := by
+      simp [h_sub, baseMro]
+    simp only [sub_baseMro]
+    intro h ty
+    cases h with
+    | inl sup_eq_sub =>
+      simp [sup_eq_sub, sub_baseMro]
+    | inr sup_mem_mro_base =>
+      simp only [← mem_mro_iff]
+      intro ty_mem
+      exact Or.inr <| sup_mem_sub sup_mem_mro_base ty_mem
+termination_by sub
+decreasing_by simp [sub_baseMro]
+
+def Subtype (self other : TypeSpecRef) : Prop :=
+  other ∈ self.mro
+
+instance : HasSubset TypeSpecRef := ⟨TypeSpecRef.Subtype⟩
+
+theorem subset_iff_mem_mro : a ⊆ b ↔ b ∈ mro a := Iff.rfl
+
+theorem subset_iff_eq_or_mem_baseMro : a ⊆ b ↔ (a = b ∨ b ∈ baseMro a) := by
+  grind [subset_iff_mem_mro, mro_def]
+
+@[simp] theorem Subtype.rfl {self : TypeSpecRef} : self ⊆ self := self_mem_mro
+
+@[simp] theorem Subtype.refl (self : TypeSpecRef) : self ⊆ self := self_mem_mro
+
+theorem Subtype.trans {a b c : TypeSpecRef} : a ⊆ b → b ⊆ c → a ⊆ c  := by
+  simp only [subset_iff_mem_mro]
+  exact fun h₁ h₂ => sup_mem_sub h₁ h₂
+
+instance : Trans (Subset : TypeSpecRef → TypeSpecRef → Prop) Subset Subset :=
+  ⟨Subtype.trans⟩
+
+@[inherit_doc TypeSpec.name]
+abbrev name (self : TypeSpecRef) : String :=
+  self.data.name
+
+@[simp, inherit_doc TypeSpec.isTypeSubclass]
+abbrev isTypeSubclass (self : TypeSpecRef) : Bool :=
+  self.data.isTypeSubclass
+
+@[simp, inherit_doc TypeSpec.isIntSubclass]
+abbrev isIntSubclass (self : TypeSpecRef) : Bool :=
+  self.data.isIntSubclass
+
+@[simp, inherit_doc TypeSpec.isStrSubclass]
+abbrev isStrSubclass (self : TypeSpecRef) : Bool :=
+  self.data.isStrSubclass
+
+@[simp, inherit_doc TypeSpec.IsValidObject]
+abbrev IsValidObject (self : TypeSpecRef) (id : ObjectId) (data : ObjectData) : Prop :=
+  self.data.IsValidObject id data
+
+end TypeSpecRef
+
+structure DTypeSpecRef (ty : TypeSpec) extends NonScalarRef TypeSpec where
+  data_eq : toNonScalarRef.data = ty
+
+namespace DTypeSpecRef
+
+attribute [simp] data_eq
+
+instance : Nonempty (DTypeSpecRef ty) := ⟨⟨.null ty, rfl⟩⟩
+
+@[inline] def toTypeSpecRef (self : DTypeSpecRef ty) : TypeSpecRef :=
+  self.toFrozenRef.cast self.data_eq
+
+@[simp] theorem isNonScalar_addr_toTypeSpecRef {self : DTypeSpecRef ty} :
+  self.toTypeSpecRef.addr % 2 = 0
+:= self.addr_mod_two
+
+end DTypeSpecRef
+
+instance : CoeOut (DTypeSpecRef ty) TypeSpecRef :=
+  ⟨DTypeSpecRef.toTypeSpecRef⟩
+
+@[inline] private unsafe def mkTypeSpecRefImpl
+  (ty : TypeSpec) : BaseIO (DTypeSpecRef ty)
+:= pure (unsafeCast ty)
+
+@[implemented_by mkTypeSpecRefImpl]
+opaque mkDTypeSpecRef (ty : TypeSpec) : BaseIO (DTypeSpecRef ty) :=
+  pure ⟨NonScalarRef.null ty, NonScalarRef.data_null⟩
+
+@[inline] def mkTypeSpecRef (ty : TypeSpec) : BaseIO TypeSpecRef := do
+  (·.toTypeSpecRef) <$> mkDTypeSpecRef ty
