tests/api.lean
@@ -4,3 +4,12 @@ open LeanPy
 
 /-- info: false -/
 #guard_msgs in #eval return (← mkObjectObject).beq (← mkObjectObject)
+
+/-- info: true -/
+#guard_msgs in #eval (intTypeRef' : Object).asObject.beq (intTypeRef' : Object)
+
+/-- info: false -/
+#guard_msgs in #eval (intTypeRef' : Object).asObject.beq (boolTypeRef' : Object)
+
+/-- info: false -/
+#guard_msgs in #eval (intTypeRef' : Object).asObject.beq (0 : Object)
